> 利用栈实现下列递归函数的非递归算法  
> Pn(x) = 1                         n = 0  
> Pn(x) = 2x                        n = 1
> Pn(x) = 2xPn-1(x) - 2(n-1)Pn-2(x) n > 1  

```cpp
double Pnx(int n, double x) {
    if (n == 0) return 1;
    double fv1 = 1, fv2 = 2 * x;
    stack<double> s;                // 借助栈来实现
    s.push(fv1);
    s.puhs(fv2);

    for (int i = 2; i <= n; ++i) {
        fv2 = s.top();  s.pop();
        fv1 = s.top();  s.pop();
        s.push(fv2);
        s.push(2*(x * fv2 - (i - 1) fv1));
    }

    return s.top();
}

```